src/CIU.v
@@ -1,0 +1,7 @@
+Require Import LogRel.
+Import ListNotations.
+
+Definition CIU (e1 e2 : Exp) : Prop :=
+  EXPCLOSED e1 /\ EXPCLOSED e2 /\
+  exists v1 v2, (* Vrel v1 v2 /\  <- here n-independent equivalence needed *)
+  (exists clock, eval clock e1 = Res v1) <-> (exists clock, eval clock e2 = Res v2). 
